solve admit in lockmap_proof using delete in new gen_heap

src/Helpers/GenHeap.v
@@ -1,8 +1,7 @@
-From stdpp Require Export namespaces.
 From iris.bi.lib Require Import fractional.
 From iris.proofmode Require Import tactics.
-From iris.algebra Require Import auth gmap frac agree namespace_map.
-From iris.base_logic.lib Require Export own gen_heap.
+From iris.algebra Require Import auth gmap frac agree.
+From iris.base_logic.lib Require Import own gen_heap.
 Set Default Proof Using "Type".
 Import uPred.
 
@@ -10,40 +9,40 @@ Import uPred.
     so that we can support deletion. *)
 
 (** The CMRA we need. *)
-Class xgen_heapG (L V : Type) (Σ : gFunctors) `{Countable L} := XGenHeapG {
-  xgen_heap_inG :> inG Σ (authR (gen_heapUR L V));
-  xgen_heap_name : gname
+Class gen_heapG (L V : Type) (Σ : gFunctors) `{Countable L} := GenHeapG {
+  gen_heap_inG :> inG Σ (authR (gen_heapUR L V));
+  gen_heap_name : gname
 }.
-Arguments xgen_heap_name {_ _ _ _ _} _ : assert.
+Arguments gen_heap_name {_ _ _ _ _} _ : assert.
 
-Class xgen_heapPreG (L V : Type) (Σ : gFunctors) `{Countable L} := {
-  xgen_heap_preG_inG :> inG Σ (authR (gen_heapUR L V))
+Class gen_heapPreG (L V : Type) (Σ : gFunctors) `{Countable L} := {
+  gen_heap_preG_inG :> inG Σ (authR (gen_heapUR L V))
 }.
 
-Definition xgen_heapΣ (L V : Type) `{Countable L} : gFunctors := #[
+Definition gen_heapΣ (L V : Type) `{Countable L} : gFunctors := #[
   GFunctor (authR (gen_heapUR L V))
 ].
 
 Instance xsubG_gen_heapPreG {Σ L V} `{Countable L} :
-  subG (xgen_heapΣ L V) Σ → xgen_heapPreG L V Σ.
+  subG (gen_heapΣ L V) Σ → gen_heapPreG L V Σ.
 Proof. solve_inG. Qed.
 
 Section definitions.
-  Context `{Countable L, hG : !xgen_heapG L V Σ}.
+  Context `{Countable L, hG : !gen_heapG L V Σ}.
 
-  Definition xgen_heap_ctx (σ : gmap L V) : iProp Σ := (
-    own (xgen_heap_name hG) (● (to_gen_heap σ)))%I.
+  Definition gen_heap_ctx (σ : gmap L V) : iProp Σ := (
+    own (gen_heap_name hG) (● (to_gen_heap σ)))%I.
 
-  Definition xmapsto_def (l : L) (q : Qp) (v: V) : iProp Σ :=
-    own (xgen_heap_name hG) (◯ {[ l := (q, to_agree (v : leibnizO V)) ]}).
-  Definition xmapsto_aux : seal (@xmapsto_def). by eexists. Qed.
-  Definition xmapsto := xmapsto_aux.(unseal).
-  Definition xmapsto_eq : @xmapsto = @xmapsto_def := xmapsto_aux.(seal_eq).
+  Definition mapsto_def (l : L) (q : Qp) (v: V) : iProp Σ :=
+    own (gen_heap_name hG) (◯ {[ l := (q, to_agree (v : leibnizO V)) ]}).
+  Definition mapsto_aux : seal (@mapsto_def). by eexists. Qed.
+  Definition mapsto := mapsto_aux.(unseal).
+  Definition mapsto_eq : @mapsto = @mapsto_def := mapsto_aux.(seal_eq).
 End definitions.
 
-Local Notation "l ↦{ q } v" := (xmapsto l q v)
+Local Notation "l ↦{ q } v" := (mapsto l q v)
   (at level 20, q at level 50, format "l  ↦{ q }  v") : bi_scope.
-Local Notation "l ↦ v" := (xmapsto l 1 v) (at level 20) : bi_scope.
+Local Notation "l ↦ v" := (mapsto l 1 v) (at level 20) : bi_scope.
 
 Local Notation "l ↦{ q } -" := (∃ v, l ↦{q} v)%I
   (at level 20, q at level 50, format "l  ↦{ q }  -") : bi_scope.
@@ -58,16 +57,16 @@ Section to_gen_heap.
   Proof. by rewrite /to_gen_heap fmap_delete. Qed.
 End to_gen_heap.
 
-Lemma xgen_heap_init `{Countable L, !xgen_heapPreG L V Σ} σ :
-  (|==> ∃ _ : xgen_heapG L V Σ, xgen_heap_ctx σ)%I.
+Lemma gen_heap_init `{Countable L, !gen_heapPreG L V Σ} σ :
+  (|==> ∃ _ : gen_heapG L V Σ, gen_heap_ctx σ)%I.
 Proof.
   iMod (own_alloc (● to_gen_heap σ)) as (γh) "Hh".
   { rewrite auth_auth_valid. exact: to_gen_heap_valid. }
-  iModIntro. iExists (XGenHeapG L V Σ _ _ _ γh). done.
+  iModIntro. iExists (GenHeapG L V Σ _ _ _ γh). done.
 Qed.
 
 Section gen_heap.
-  Context {L V} `{Countable L, !xgen_heapG L V Σ}.
+  Context {L V} `{Countable L, !gen_heapG L V Σ}.
   Implicit Types P Q : iProp Σ.
   Implicit Types Φ : V → iProp Σ.
   Implicit Types σ : gmap L V.
@@ -76,60 +75,60 @@ Section gen_heap.
   Implicit Types v : V.
 
   (** General properties of mapsto *)
-  Global Instance xmapsto_timeless l q v : Timeless (l ↦{q} v).
-  Proof. rewrite xmapsto_eq /xmapsto_def. apply _. Qed.
-  Global Instance xmapsto_fractional l v : Fractional (λ q, l ↦{q} v)%I.
+  Global Instance mapsto_timeless l q v : Timeless (l ↦{q} v).
+  Proof. rewrite mapsto_eq /mapsto_def. apply _. Qed.
+  Global Instance mapsto_fractional l v : Fractional (λ q, l ↦{q} v)%I.
   Proof.
-    intros p q. by rewrite xmapsto_eq /xmapsto_def -own_op -auth_frag_op
+    intros p q. by rewrite mapsto_eq /mapsto_def -own_op -auth_frag_op
       op_singleton -pair_op agree_idemp.
   Qed.
-  Global Instance xmapsto_as_fractional l q v :
+  Global Instance mapsto_as_fractional l q v :
     AsFractional (l ↦{q} v) (λ q, l ↦{q} v)%I q.
   Proof. split. done. apply _. Qed.
 
-  Lemma xmapsto_agree l q1 q2 v1 v2 : l ↦{q1} v1 -∗ l ↦{q2} v2 -∗ ⌜v1 = v2⌝.
+  Lemma mapsto_agree l q1 q2 v1 v2 : l ↦{q1} v1 -∗ l ↦{q2} v2 -∗ ⌜v1 = v2⌝.
   Proof.
     apply wand_intro_r.
-    rewrite xmapsto_eq /xmapsto_def -own_op -auth_frag_op own_valid discrete_valid.
+    rewrite mapsto_eq /mapsto_def -own_op -auth_frag_op own_valid discrete_valid.
     f_equiv. rewrite auth_frag_valid op_singleton singleton_valid -pair_op.
     by intros [_ ?%agree_op_invL'].
   Qed.
 
-  Lemma xmapsto_combine l q1 q2 v1 v2 :
+  Lemma mapsto_combine l q1 q2 v1 v2 :
     l ↦{q1} v1 -∗ l ↦{q2} v2 -∗ l ↦{q1 + q2} v1 ∗ ⌜v1 = v2⌝.
   Proof.
-    iIntros "Hl1 Hl2". iDestruct (xmapsto_agree with "Hl1 Hl2") as %->.
+    iIntros "Hl1 Hl2". iDestruct (mapsto_agree with "Hl1 Hl2") as %->.
     iCombine "Hl1 Hl2" as "Hl". eauto with iFrame.
   Qed.
 
-  Global Instance ex_xmapsto_fractional l : Fractional (λ q, l ↦{q} -)%I.
+  Global Instance ex_mapsto_fractional l : Fractional (λ q, l ↦{q} -)%I.
   Proof.
     intros p q. iSplit.
     - iDestruct 1 as (v) "[H1 H2]". iSplitL "H1"; eauto.
     - iIntros "[H1 H2]". iDestruct "H1" as (v1) "H1". iDestruct "H2" as (v2) "H2".
-      iDestruct (xmapsto_agree with "H1 H2") as %->. iExists v2. by iFrame.
+      iDestruct (mapsto_agree with "H1 H2") as %->. iExists v2. by iFrame.
   Qed.
-  Global Instance ex_xmapsto_as_fractional l q :
+  Global Instance ex_mapsto_as_fractional l q :
     AsFractional (l ↦{q} -) (λ q, l ↦{q} -)%I q.
   Proof. split. done. apply _. Qed.
 
-  Lemma xmapsto_valid l q v : l ↦{q} v -∗ ✓ q.
+  Lemma mapsto_valid l q v : l ↦{q} v -∗ ✓ q.
   Proof.
-    rewrite xmapsto_eq /xmapsto_def own_valid !discrete_valid -auth_frag_valid.
+    rewrite mapsto_eq /mapsto_def own_valid !discrete_valid -auth_frag_valid.
     by apply pure_mono=> /singleton_valid [??].
   Qed.
-  Lemma xmapsto_valid_2 l q1 q2 v1 v2 : l ↦{q1} v1 -∗ l ↦{q2} v2 -∗ ✓ (q1 + q2)%Qp.
+  Lemma mapsto_valid_2 l q1 q2 v1 v2 : l ↦{q1} v1 -∗ l ↦{q2} v2 -∗ ✓ (q1 + q2)%Qp.
   Proof.
-    iIntros "H1 H2". iDestruct (xmapsto_agree with "H1 H2") as %->.
-    iApply (xmapsto_valid l _ v2). by iFrame.
+    iIntros "H1 H2". iDestruct (mapsto_agree with "H1 H2") as %->.
+    iApply (mapsto_valid l _ v2). by iFrame.
   Qed.
 
   (** Update lemmas *)
-  Lemma xgen_heap_alloc σ l v :
+  Lemma gen_heap_alloc σ l v :
     σ !! l = None →
-    xgen_heap_ctx σ ==∗ xgen_heap_ctx (<[l:=v]>σ) ∗ l ↦ v.
+    gen_heap_ctx σ ==∗ gen_heap_ctx (<[l:=v]>σ) ∗ l ↦ v.
   Proof.
-    iIntros (Hσl). rewrite /xgen_heap_ctx xmapsto_eq /xmapsto_def /=.
+    iIntros (Hσl). rewrite /gen_heap_ctx mapsto_eq /mapsto_def /=.
     iIntros "Hσ".
     iMod (own_update with "Hσ") as "[Hσ Hl]".
     { eapply auth_update_alloc,
@@ -139,32 +138,32 @@ Section gen_heap.
     rewrite to_gen_heap_insert //.
   Qed.
 
-  Lemma xgen_heap_alloc_gen σ σ' :
+  Lemma gen_heap_alloc_gen σ σ' :
     σ' ##ₘ σ →
-    xgen_heap_ctx σ ==∗
-    xgen_heap_ctx (σ' ∪ σ) ∗ ([∗ map] l ↦ v ∈ σ', l ↦ v).
+    gen_heap_ctx σ ==∗
+    gen_heap_ctx (σ' ∪ σ) ∗ ([∗ map] l ↦ v ∈ σ', l ↦ v).
   Proof.
     revert σ; induction σ' as [| l v σ' Hl IH] using map_ind; iIntros (σ Hdisj) "Hσ".
     { rewrite left_id_L. auto. }
     iMod (IH with "Hσ") as "[Hσ'σ Hσ']"; first by eapply map_disjoint_insert_l.
     decompose_map_disjoint.
     rewrite !big_opM_insert // -insert_union_l //.
-    by iMod (xgen_heap_alloc with "Hσ'σ") as "($ & $)";
+    by iMod (gen_heap_alloc with "Hσ'σ") as "($ & $)";
       first by apply lookup_union_None.
   Qed.
 
-  Lemma xgen_heap_valid σ l q v : xgen_heap_ctx σ -∗ l ↦{q} v -∗ ⌜σ !! l = Some v⌝.
+  Lemma gen_heap_valid σ l q v : gen_heap_ctx σ -∗ l ↦{q} v -∗ ⌜σ !! l = Some v⌝.
   Proof.
     iIntros "Hσ Hl".
-    rewrite /xgen_heap_ctx xmapsto_eq /xmapsto_def.
+    rewrite /gen_heap_ctx mapsto_eq /mapsto_def.
     iDestruct (own_valid_2 with "Hσ Hl")
       as %[Hl%gen_heap_singleton_included _]%auth_both_valid; auto.
   Qed.
 
-  Lemma xgen_heap_update σ l v1 v2 :
-    xgen_heap_ctx σ -∗ l ↦ v1 ==∗ xgen_heap_ctx (<[l:=v2]>σ) ∗ l ↦ v2.
+  Lemma gen_heap_update σ l v1 v2 :
+    gen_heap_ctx σ -∗ l ↦ v1 ==∗ gen_heap_ctx (<[l:=v2]>σ) ∗ l ↦ v2.
   Proof.
-    iIntros "Hσ Hl". rewrite /xgen_heap_ctx xmapsto_eq /xmapsto_def.
+    iIntros "Hσ Hl". rewrite /gen_heap_ctx mapsto_eq /mapsto_def.
     iDestruct (own_valid_2 with "Hσ Hl")
       as %[Hl%gen_heap_singleton_included _]%auth_both_valid.
     iMod (own_update_2 with "Hσ Hl") as "[Hσ Hl]".
@@ -174,12 +173,12 @@ Section gen_heap.
     iModIntro. iFrame "Hl". rewrite to_gen_heap_insert //.
   Qed.
 
-  Lemma xgen_heap_delete σ l v :
-    l ↦ v ∗ xgen_heap_ctx σ ==∗ xgen_heap_ctx (delete l σ).
+  Lemma gen_heap_delete σ l v :
+    l ↦ v ∗ gen_heap_ctx σ ==∗ gen_heap_ctx (delete l σ).
   Proof.
     iIntros "[Hl Hσ]".
-    iDestruct (xgen_heap_valid with "Hσ Hl") as %?.
-    rewrite /xgen_heap_ctx xmapsto_eq /xmapsto_def /=.
+    iDestruct (gen_heap_valid with "Hσ Hl") as %?.
+    rewrite /gen_heap_ctx mapsto_eq /mapsto_def /=.
     iMod (own_update with "[Hl Hσ]") as "Hσ".
     2: iApply own_op; iFrame.
     { eapply auth_update_dealloc.
